prove that product is same as merging prime factors

Alg/ListProps/Sorted/Merge.lean
@@ -1,70 +1,299 @@
-import Alg.ListProps.Sorted
+import Alg.ListProps.Sorted.Induction
 
-def List.sorted_merge [Compare α] (as bs: List α) := match as with
-  | [] => bs
-  | a::as' => as'.sorted_merge (bs.sorted_push a)
+def List.sorted_merge [Compare α] (as bs: List α) := by
+  apply sorted.induction
+  {
+    intro bs
+    exact bs
+  }
+  {
+    intro a as
+    exact a::as
+  }
+  {
+    intro a _ b _ _ prev
+    exact a::prev
+  }
+  {
+    intro a _ b _ _ prev
+    exact a::b::prev
+  }
+  {
+    intro a _ b _ _ prev
+    exact b::prev
+  }
 
-  def List.sorted_merge.keeps_sorted [Compare α] (as bs: List α) : as.sorted -> bs.sorted -> (as.sorted_merge bs).sorted := by
-    intro as_sorted bs_sorted
-    match as with
-    | [] =>
-      unfold List.sorted_merge
-      exact bs_sorted
-    | a::as' =>
-      unfold List.sorted_merge
-      apply List.sorted_merge.keeps_sorted
-      apply List.sorted.pop
+theorem List.sorted_merge.empty_left [Compare α] : ∀{bs: List α}, [].sorted_merge bs = bs := by
+  intro bs
+  apply List.sorted.empty_left
+
+#print axioms List.sorted_merge.empty_left
+
+theorem List.sorted_merge.empty_right [Compare α] : ∀{as: List α}, as.sorted_merge [] = as := by
+  intro as
+  cases as
+  rfl
+  apply List.sorted.empty_right
+
+#print axioms List.sorted_merge.empty_right
+
+theorem List.sorted_merge.induct_lt [Compare α] : ∀{a b: α} {as bs: List α}, Compare.ord a b = Order.Less -> (a::as).sorted_merge (b::bs) = a::(as.sorted_merge (b::bs)) := by
+  apply List.sorted.induct_lt
+
+#print axioms List.sorted_merge.induct_lt
+
+theorem List.sorted_merge.induct_eq [Compare α] : ∀{a b: α} {as bs: List α}, Compare.ord a b = Order.Eq -> (a::as).sorted_merge (b::bs) = a::b::(as.sorted_merge bs) := by
+  apply List.sorted.induct_eq
+
+#print axioms List.sorted_merge.induct_lt
+
+theorem List.sorted_merge.induct_gt [Compare α] : ∀{a b: α} {as bs: List α}, Compare.ord a b = Order.Greater -> (a::as).sorted_merge (b::bs) = b::((a::as).sorted_merge bs) := by
+  apply List.sorted.induct_gt
+
+#print axioms List.sorted_merge.induct_gt
+
+theorem List.sorted_merge.keeps_sorted.helper [Compare α] {x: α} : 
+  ∀ {as bs},
+  sorted (x::as) ->
+  sorted (x::bs) ->
+  sorted (sorted_merge as bs) ->
+  sorted (x :: sorted_merge as bs) := by
+  apply sorted.induction
+  {
+    intro _
+    intro _ _ _
+    rw [empty_left]
+    assumption
+  }
+  {
+    intro _ _
+    intro _ _ _
+    rw [empty_right]
+    assumption
+  }
+  {
+    intro a as b bs a_ord_b _
+    intro as_sort _ i_sort
+    rw [induct_lt a_ord_b]
+    rw [induct_lt a_ord_b] at i_sort
+    apply And.intro
+    exact as_sort.left
+    assumption
+  }
+  {
+    intro a as b bs a_ord_b _
+    intro as_sort _ i_sort
+    rw [induct_eq a_ord_b]
+    rw [induct_eq a_ord_b] at i_sort
+    apply And.intro
+    exact as_sort.left
+    assumption
+  }
+  {
+    intro a as b bs a_ord_b _
+    intro _ bs_sort i_sort
+    rw [induct_gt a_ord_b]
+    rw [induct_gt a_ord_b] at i_sort
+    apply And.intro
+    exact bs_sort.left
+    assumption
+  }
+
+theorem List.sorted_merge.keeps_sorted [Compare α] : ∀(as bs: List α), as.sorted -> bs.sorted -> (as.sorted_merge bs).sorted := by
+    apply sorted.induction
+    {
+      intro bss
+      intro _ _
+      rw [empty_left]
       assumption
-      apply List.sorted_push.keeps_sorted
+    }
+    {
+      intro a as
+      intro _ _
+      rw [empty_right]
       assumption
+    }
+    {
+      intro a as b bs a_ord_b prev
+      intro as_sort bs_sort
+      rw [induct_lt a_ord_b]
+      apply List.sorted_merge.keeps_sorted.helper
+      any_goals assumption
+      apply And.intro
+      apply Or.inl
+      exact a_ord_b
+      assumption
+      apply prev
+      exact as_sort.pop
+      assumption
+    }
+    {
+      intro a as b bs a_ord_b prev
+      intro as_sort bs_sort
+      rw [induct_eq a_ord_b]
+      apply And.intro
+      apply Or.inr
+      assumption
+      apply List.sorted_merge.keeps_sorted.helper
+      any_goals assumption
+      rw [←(Compare.ord_to_eq a_ord_b)]
+      assumption
+      apply prev
+      exact as_sort.pop
+      exact bs_sort.pop
+    }
+    {
+      intro a as b bs a_ord_b prev
+      intro as_sort bs_sort
+      rw [induct_gt a_ord_b]
+      apply List.sorted_merge.keeps_sorted.helper
+      any_goals assumption
+      apply And.intro
+      apply Or.inl
+      exact Compare.flip a_ord_b
+      assumption
+      apply prev
+      assumption
+      exact bs_sort.pop
+    }
+    repeat admit
 
 #print axioms List.sorted_merge.keeps_sorted
 
-  def List.sorted_merge.keeps_allP {P: α -> Prop} [Compare α] (as bs: List α) : as.allP P -> bs.allP P -> (as.sorted_merge bs).allP P := by
-    intro as_all bs_all
-    match as with
-    | [] =>
-      unfold List.sorted_merge
-      exact bs_all
-    | a::as' =>
-      unfold List.sorted_merge
-      apply List.sorted_merge.keeps_allP
-      exact as_all.right
-      apply List.sorted_push.keeps_allP
+theorem List.sorted_merge.keeps_allP {P: α -> Prop} [Compare α] : ∀{as bs: List α}, as.allP P -> bs.allP P -> (as.sorted_merge bs).allP P := by
+    apply sorted.induction
+    {
+      intro bs
+      intro _ bs_all
+      rw [empty_left]
       assumption
+    }
+    {
+      intro a as
+      intro as_all _
+      rw [empty_right]
+      assumption
+    }
+    {
+      intro a as b bs a_ord_b prev
+      intro as_all bs_all
+      rw [induct_lt a_ord_b]
+      apply And.intro
       exact as_all.left
+      apply prev
+      exact as_all.right
+      assumption
+    }
+    {
+      intro a as b bs a_ord_b prev
+      intro as_all bs_all
+      rw [induct_eq a_ord_b]
+      apply And.intro
+      exact as_all.left
+      apply And.intro
+      exact bs_all.left
+      apply prev
+      exact as_all.right
+      exact bs_all.right
+    }
+    {
+      intro a as b bs a_ord_b prev
+      intro as_all bs_all
+      rw [induct_gt a_ord_b]
+      apply And.intro
+      exact bs_all.left
+      apply prev
+      assumption
+      exact bs_all.right
+    }
 
 #print axioms List.sorted_merge.keeps_allP
 
-  def List.sorted_merge.keeps_anyP {P: α -> Prop} [Compare α] (as bs: List α) : as.anyP P ∨ bs.anyP P -> (as.sorted_merge bs).anyP P := by
-    intro as_any_or_bs_any
-    match as with
-    | [] =>
-      unfold List.sorted_merge
-      match as_any_or_bs_any with
+theorem List.sorted_merge.keeps_anyP {P: α -> Prop} [Compare α] : ∀{as bs: List α}, as.anyP P ∨ bs.anyP P -> (as.sorted_merge bs).anyP P := by
+    apply sorted.induction
+    {
+      intro bs
+      intro as_or_bs
+      rw [empty_left]
+      match as_or_bs with
       | .inl _ => contradiction
-      | .inr h => assumption
-    | a::as' =>
-      unfold List.sorted_merge
-      apply List.sorted_merge.keeps_anyP
-      match as_any_or_bs_any with
-      | .inl (.inr _) =>
+      | .inr _ => assumption
+    }
+    {
+      intro a as
+      intro as_or_bs
+      rw [empty_right]
+      match as_or_bs with
+      | .inl _ => assumption
+      | .inr _ => contradiction
+    }
+    {
+      intro a as b bs a_ord_b prev
+      intro as_or_bs
+      rw [induct_lt a_ord_b]
+      match as_or_bs with
+      | .inl (.inl _) =>
         apply Or.inl
         assumption
-      | .inl (.inl _) =>
+      | .inl (.inr _) =>
         apply Or.inr
-        apply List.sorted_push.keeps_anyP
-        apply Or.inr
+        apply prev
+        apply Or.inl
         assumption
       | .inr _ =>
         apply Or.inr
-        apply List.sorted_push.keeps_anyP
+        apply prev
+        apply Or.inr
+        assumption
+    }
+    {
+      intro a as b bs a_ord_b prev
+      intro as_or_bs
+      rw [induct_eq a_ord_b]
+      match as_or_bs with
+      | .inl (.inl _) =>
         apply Or.inl
         assumption
+      | .inl (.inr _) =>
+        apply Or.inr
+        apply Or.inr
+        apply prev
+        apply Or.inl
+        assumption
+      | .inr (.inl _) =>
+        apply Or.inl
+        rw [Compare.ord_to_eq a_ord_b]
+        assumption
+      | .inr (.inr _) =>
+        apply Or.inr
+        apply Or.inr
+        apply prev
+        apply Or.inr
+        assumption
+    }
+    {
+      intro a as b bs a_ord_b prev
+      intro as_or_bs
+      rw [induct_gt a_ord_b]
+      match as_or_bs with
+      | .inr (.inl _) =>
+        apply Or.inl
+        assumption
+      | .inr (.inr _) =>
+        apply Or.inr
+        apply prev
+        apply Or.inr
+        assumption
+      | .inl _ =>
+        apply Or.inr
+        apply prev
+        apply Or.inl
+        assumption
+    }
 
 #print axioms List.sorted_merge.keeps_anyP
 
-  def List.sorted_merge.contains [Compare α] (as bs: List α) (x: α) : as.containsP x ∨ bs.containsP x -> (as.sorted_merge bs).containsP x := by
+def List.sorted_merge.contains [Compare α] (as bs: List α) (x: α) : as.containsP x ∨ bs.containsP x -> (as.sorted_merge bs).containsP x := by
     unfold containsP
     apply List.sorted_merge.keeps_anyP
 
